coq/List.v
@@ -1,0 +1,74 @@
+Require Import Coq.Lists.List.
+Require ssreflect.
+
+Require Import Coq.Classes.RelationClasses.
+Require Import Coq.Relations.Relation_Definitions.
+
+(* List Library functions. *)
+
+Inductive ExistsT {A : Type} (P : A -> Type) : list A -> Type :=
+  | ExistsT_cons1 : forall (x : A) (l : list A), 
+      P x  -> ExistsT P (x :: l)
+  | ExistsT_cons2 : forall (x : A) (l : list A), 
+      ExistsT P l -> ExistsT P (x :: l).
+
+Inductive Exists2 {A B : Type} (P : A -> B -> Prop) : 
+  list A -> list B -> Prop :=
+    Exists2_cons_hd : forall x y l l',
+      P x y -> Exists2 P (x :: l) (y :: l')
+  | Exists2_cons_tl : forall x y l l', 
+      Exists2 P l l' -> Exists2 P (x :: l) (y :: l').
+
+#[export] Hint Constructors ExistsT Exists2 : core.
+
+Inductive ForallT {A : Type} (P : A -> Type) : list A -> Type :=
+    ForallT_nil : ForallT P nil
+  | ForallT_cons : forall (x : A) (l : list A), P x -> ForallT P l -> ForallT P (x :: l).
+
+#[export] Hint Constructors ForallT : core.
+
+
+(* Properties of Forall2 *)
+
+Lemma Forall_Forall2 {A} {P : A -> A -> Prop} l : 
+  Forall (fun x : A => P x x) l <->
+  Forall2 P l l.
+Proof.
+  induction l; split; intro h; inversion h; subst; eauto.
+  econstructor; eauto. rewrite <- IHl. auto.
+  econstructor; eauto. rewrite -> IHl. auto.
+Qed.
+
+#[export] Instance Reflexive_Forall2 {A}{P: A -> A -> Prop}`{Reflexive _ P} : Reflexive (Forall2 P).
+Proof.
+  intros.
+  intros l. induction l; eauto.
+Qed.
+
+#[export] Instance Symmetric_Forall2 {A}{P: A -> A -> Prop}`{Symmetric _ P} : Symmetric (Forall2 P).
+Proof.
+  intros x y F.
+  induction F; eauto.
+Qed.
+
+#[export] Instance Transitive_Forall2 {A}{P: A -> A -> Prop}`{Transitive _ P} : Transitive (Forall2 P).
+Proof.
+  intros x y.
+  generalize x. clear x. 
+  induction y; intros x z F1 F2;
+  inversion F1; inversion F2; subst; eauto.
+Qed.
+
+
+Lemma Forall2_length {A} {P : A -> A -> Prop} l1 l2 : 
+  Forall2 P l1 l2 -> 
+  length l1 = length l2.
+Proof.
+  generalize l2. clear l2.
+  induction l1; intros l2 h;
+  inversion h; subst; simpl in *; eauto.
+Qed.  
+
+Lemma Exists_Exists2 : forall {A} (P : A -> A -> Prop) (l:list A), 
+    Exists (fun x => P x x) l <-> Exists2 P l l.
+Admitted. 
